B-unification/lowenheim.v
@@ -84,16 +84,42 @@ intros. unfold unifier in *. induction sigma.
   simpl in *. 
 Admitted.
 
-Lemma lowenheim_subst_generates_unifiers :
-  forall (t : term) (sigma : subst) , unifier t sigma -> unifier t (lowenheim_subst t sigma).
+Lemma subst_lowenheim_subst_equiv :
+  forall (sigma : subst) (t : term),
+  apply_subst t sigma == apply_subst t (lowenheim_subst t sigma).
 Proof.
-intros. induction sigma.
+intro. induction sigma.
 {
-  simpl in *. apply H.
+  intros. simpl. reflexivity.
 }
 {
-Admitted.
+  intros. simpl. induction t.
+  {
+    simpl. apply IHsigma.
+  }
+  {
+    simpl. apply IHsigma.
+  }
+  {
+    simpl. 
+Admitte.
 
+Lemma lowenheim_subst_generates_unifiers :
+  forall (t : term) (sigma : subst), unifier t sigma <-> unifier t (lowenheim_subst t sigma).
+Proof.
+intros. split.
+{ 
+  intros. unfold unifier in *. rewrite <- subst_lowenheim_subst_equiv. apply H.
+}
+{
+  intros. unfold unifier in *. rewrite subst_lowenheim_subst_equiv. apply H.
+}
+Qed.
+
+Lemma lowenheim_subst_generates_mgus :
+  forall (t : term) (sigma : subst), unifier t sigma -> mgu t (lowenheim_subst t sigma).
+Proof.
+Admitted.
 
 
 
